\documentclass[a4paper,12pt]{article}
\usepackage{graphicx}
\usepackage{amsmath}
\title{Assignment-2\\ Latex Report}
\author{Fuzayil Bin Afzal Mir}
\date{13/01/2021}
\begin{document}
	\maketitle
	
	
	\newpage
	\begin{itemize}
	    \item \Large\textbf{Exercise 2.54}
	\end{itemize}
	\section{Find X and Y, If 
	X+Y =	\begin{pmatrix}
		 5 & 2\\
		 0 & 9\\
	\end{pmatrix}
	and \\
	X-Y = \begin{pmatrix}
		3 & 6\\
	    0 & -1\\
	\end{pmatrix}
}









	\subsection{Solution} \\
	Giving equation number to the given equations,\\
	So let

	
	
	\begin{equation}\label{eq1}
	    \begin{split}
	        		X+Y =	\begin{pmatrix}
		 5 & 2\\
		 0 & 9\\
	\end{pmatrix}	
	    \end{split}
	\end{equation}
	

	and 
	
	
	
	\begin{equation}\label{eq1}
	    \begin{split}
		X-Y = \begin{pmatrix}
		3 & 6\\
	    0 & -1\\
	\end{pmatrix}
	\end{split}
	\end{equation}
	
Now,\\$$$$\\
Adding eq(1) and eq(2)\\$$$$\\
X+Y+(X-Y)=	\begin{pmatrix}
		 5 & 2\\
		 0 & 9\\
	\end{pmatrix}
	+
	\begin{pmatrix}
		3 & 6\\
	    0 & -1\\
	\end{pmatrix}\\$$$$\\

X+Y+X-Y=\begin{pmatrix}
		 8 & 8\\
		 0 & 8\\
	\end{pmatrix}\\$$$$\\
	
		2X+0Y=\begin{pmatrix}
		 8 & 8\\
		 0 & 8\\
	\end{pmatrix}\\$$$$\\
	Or,
	
	2X=\begin{pmatrix}
		 8 & 8\\
		 0 & 8\\
	\end{pmatrix}\\$$$$\\
	
	\begin{gather}
	X= \frac{1}{2}
	\begin{pmatrix}
		 8 & 8\\
		 0 & 8\\
	\end{pmatrix}\\
	\end{gather}\\$$$\\
	\textbf{\underline{Note: Scaler Multiplication:}}\\
	If a matrix is multiplied by a constant K,then each element of that particular matrix are multiplied by the constant K to get the resulting matrix.\\$$\\
	
	Similarly multiplying all the elements of the corresponding matrix by \dfrac{1}{2}\\$$$$\\
	
	we get,\\$$$$\\
	
	X=\begin{pmatrix}
		 \frac{8}{2} & \frac{8}{2}\\
		             &            \\
		 \frac{0}{2} & \frac{8}{2}\\
	\end{pmatrix}\\$$$$\\
	X=\begin{pmatrix}
		 4 & 4\\
		 0 & 4\\
	\end{pmatrix}\\$$$$\\
	
	
	Since we found the value of X,we will substitute this value of X in equation (1)\\$$$\\
	The equation(1) is:
		X+Y =	\begin{pmatrix}
		 5 & 2\\
		 0 & 9\\
	\end{pmatrix}\\$$$$\\
	Now after substituting value of X\\
	
		\begin{pmatrix}
		 4 & 4\\
		 0 & 4\\
	\end{pmatrix}+Y =	\begin{pmatrix}
		 5 & 2\\
		 0 & 9\\
	\end{pmatrix}\\$$$$\\
	Y=	\begin{pmatrix}
		 5 & 2\\
		 0 & 9\\
	\end{pmatrix}-
		\begin{pmatrix}
		 4 & 4\\
		 0 & 4\\
	\end{pmatrix}\\$$$\\


    Hence,\\
    \fbox{Y=	\begin{pmatrix}
		 1 & -2\\
		 0 & 5\\
	\end{pmatrix}}\\$$$$\\
    Also,\\$$$$\\
    \fbox{X=\begin{pmatrix}
		 4 & 4\\
		 0 & 4\\
	\end{pmatrix}}\\$$$$\\\vfill\emph{P.T.O}\\$$$\\
	\\$$$$\\
    \newpage
    \begin{itemize}
	    \item \Large\textbf{Exercise 2.55}
	\end{itemize}
    \section{Find the values of  x and y from the following equation:\\
    2	\begin{pmatrix}
		 x & 5\\
		 7 & y-3\\
	\end{pmatrix}
	+
	\begin{pmatrix}
		3 & -4\\
	    1 & 2\\
	\end{pmatrix}=
	\begin{pmatrix}
		7 & 6\\
	    15 & 14\\
	\end{pmatrix}}
    \subsection{Solution:}
    2	\begin{pmatrix}
		 x & 5\\
		 7 & y-3\\
	\end{pmatrix}
	+
	\begin{pmatrix}
		3 & -4\\
	    1 & 2\\
	\end{pmatrix}=
	\begin{pmatrix}
		7 & 6\\
	    15 & 14\\
	\end{pmatrix}
	
	\\$$$$\\
	\textbf{\underline{Note: Scaler Multiplication:}}\\
	If a matrix is multiplied by a constant K,then each element of that particular matrix are multiplied by the constant K to get the resulting matrix.\\$$\\
	
	Similarly multiplying 2 to all elements of the corresponding matrix.\\$$$$\\
	we get,\\$$$$\\
	\begin{pmatrix}
		 2x & 10\\
		 14 & 2(y-3)\\
	\end{pmatrix}
	+
	\begin{pmatrix}
		3 & -4\\
	    1 & 2\\
	\end{pmatrix}=
	\begin{pmatrix}
		7 & 6\\
	    15 & 14\\
	\end{pmatrix}\\$$$$\\
     	\begin{pmatrix}
		 2x & 10\\
		 14 & 2y-6\\
	\end{pmatrix}
	+
	\begin{pmatrix}
		3 & -4\\
	    1 & 2\\
	\end{pmatrix}=
	\begin{pmatrix}
		7 & 6\\
	    15 & 14\\
	\end{pmatrix}\\$$$$\\
		\begin{pmatrix}
		 2x+3 & 10+(-4)\\
		 14+1 & (2y-6)+2\\
	\end{pmatrix}
	=
	\begin{pmatrix}
		7 & 6\\
	    15 & 14\\
	\end{pmatrix}\\$$$$\\
		\begin{pmatrix}
		 2x+3 & 6\\
		 15 & 2y-4\\
	\end{pmatrix}
	=
	\begin{pmatrix}
		7 & 6\\
	    15 & 14\\
	\end{pmatrix}\\$$$$\\
Now, we get
	\begin{equation}\label{eq1}
	    \begin{split}
	      2x+3=7  
	    \end{split}
	\end{equation}
	
	and

\begin{equation}\label{eq1}
	    \begin{split}
	      2y-4=14  
	    \end{split}
	\end{equation}
	
	Using equation(5) we get,\\
	 2x=7-3\\
	 2x=4\\
	 \\
	 x=\dfrac{4}{2}\\$$$\\
	 \fbox{x=2}\\$$$\\
	 2y=14+4\\
	 2y=18\\
	 y=\dfrac{18}{2}\\$$$\\
	\fbox{y=9}\\$$$\\
	\textbf{Hence, the we got the values x=2 and y=9.}\\$$$$$$$$$$$\\
	\vfill\emph{The End}
	
\end{document}